Seperated into files.

Combinators.v
@@ -2,11 +2,11 @@ Require Import List.
 Import ListNotations.
 Require Vector Fin.
 
-Require Import Core.
-Require Import BasicSerializers.
-Require Import DeserializerMonad.
+Require Import Cheerios.Core.
+Require Import Cheerios.BasicSerializers.
+Require Import Cheerios.DeserializerMonad.
 Import DeserializerNotations.
-Require Import Tactics.
+Require Import Cheerios.Tactics.
 
 (* These functions are either missing obvious implicits, or have
    implicit arguments that are not marked "maximally inserted", which
@@ -17,6 +17,7 @@ Arguments option_map {_ _} _ _.
 Arguments Vector.nil {_}.
 Arguments Vector.cons {_} _ {_} _.
 
+Section combinators.
 
 (* This section gives instances for various type constructors, including pairs
    and lists. *)
@@ -44,12 +45,11 @@ Proof.
   destruct a; serialize_deserialize_id_crush.
 Qed.
 
-Instance option_Serializer : Serializer (option A) :=
+Global Instance option_Serializer : Serializer (option A) :=
   {| serialize := option_serialize;
       deserialize := option_deserialize;
       serialize_deserialize_id := option_serialize_deserialize_id
   |}.
-
 
 Definition pair_serialize (x : A * B) : list bool :=
   let (a, b) := x in serialize a ++ serialize b.
@@ -165,3 +165,135 @@ Global Instance vector_Serializer n : Serializer (Vector.t A n) :=
       deserialize := vector_deserialize;
       serialize_deserialize_id := vector_serialize_deserialize_id n
   |}.
+
+End combinators.
+
+Section morphism_combinators.
+  
+  Variables A B : Type.
+  Variable sA : Serializer A.
+  Variable sB : Serializer B.
+  Variable m : SerializerMorphism sA sB.
+
+  Lemma option_triangle : triangle_spec (option_map map).
+  Proof.
+    simpl.
+    unfold option_deserialize, option_serialize.
+    destruct a; triangle_crush.
+  Qed.
+
+  Global Instance option_Morphism : @SerializerMorphism (option A) (option B) _ _ :=
+    {| map := option_map map;
+        triangle := option_triangle
+    |}.
+
+
+  Variables C : Type.
+  Variable sC : Serializer C.
+
+
+  Definition pair_l_map (f : A -> B) (x : A * C) : B * C :=
+    let (a, c) := x in (f a, c).
+
+  Lemma pair_l_triangle : triangle_spec (pair_l_map map).
+  Proof.
+    simpl.
+    unfold pair_deserialize, pair_serialize.
+    destruct a; triangle_crush.
+  Qed.
+
+  Global Instance pair_l_Morphism : @SerializerMorphism (A * C) (B * C) _ _ :=
+    {| map := pair_l_map map;
+        triangle := pair_l_triangle
+    |}.
+
+
+  Definition pair_r_map (f : A -> B) (x : C * A) : C * B :=
+    let (c, a) := x in (c, f a).
+
+  Lemma pair_r_triangle : triangle_spec (pair_r_map map).
+  Proof.
+    simpl.
+    unfold pair_deserialize, pair_serialize.
+    destruct a; triangle_crush.
+  Qed.
+
+  Global Instance pair_r_Morphism : @SerializerMorphism (C * A) (C * B) _ _ :=
+    {| map := pair_r_map map;
+        triangle := pair_r_triangle
+    |}.
+
+
+  Definition sum_l_map (f : A -> B) (x : A + C) : B + C :=
+    match x with
+    | inl a => inl (f a)
+    | inr c => inr c
+    end.
+
+  Lemma sum_l_triangle : triangle_spec (sum_l_map map).
+  Proof.
+    simpl.
+    unfold sum_serialize, sum_deserialize.
+    destruct a; triangle_crush.
+  Qed.
+
+  Global Instance sum_l_Morphism : @SerializerMorphism (A + C) (B + C) _ _ :=
+    {| map := sum_l_map map;
+        triangle := sum_l_triangle
+    |}.
+
+
+  Definition sum_r_map (f : A -> B) (x : C + A) : C + B :=
+    match x with
+    | inl c => inl c
+    | inr a => inr (f a)
+    end.
+
+  Lemma sum_r_triangle : triangle_spec (sum_r_map map).
+  Proof.
+    simpl.
+    unfold sum_serialize, sum_deserialize.
+    destruct a; triangle_crush.
+  Qed.
+
+  Global Instance sum_r_Morphism : @SerializerMorphism (C + A) (C + B) _ _ :=
+    {| map := sum_r_map map;
+        triangle := sum_r_triangle
+    |}.
+
+
+  Lemma list_triangle_rec:
+    forall (a : list A) (bin : list bool),
+      list_deserialize_rec B sB (length a) (list_serialize_rec A sA a ++ bin) =
+      Some (List.map map a, bin).
+  Proof.
+    induction a; simpl; triangle_crush.
+    now rewrite IHa.
+  Qed.
+
+  Lemma list_triangle : triangle_spec (@List.map A B map).
+  Proof.
+    simpl.
+    unfold list_deserialize, list_serialize.
+    serialize_deserialize_id_crush.
+    apply list_triangle_rec.
+  Qed.
+
+  Global Instance list_morphism : @SerializerMorphism (list A) (list B) _ _ :=
+    {| map := List.map map;
+        triangle := list_triangle
+    |}.
+
+
+  Lemma vector_triangle : forall n, triangle_spec (@Vector.map A B map n).
+  Proof.
+    induction a; simpl in *; triangle_crush.
+    now rewrite IHa.
+  Qed.
+
+  Global Instance vector_morphism n : @SerializerMorphism (Vector.t A n) (Vector.t B n) _ _ :=
+    {| map := Vector.map map;
+        triangle := vector_triangle n
+    |}.
+  
+End morphism_combinators.
