Tactics.v
@@ -1,7 +1,7 @@
 Require Import List.
 
-Require Import Core.
-Require Import DeserializerMonad.
+Require Import Cheerios.Core.
+Require Import Cheerios.DeserializerMonad.
 
 Ltac deserializer_unfold :=
   unfold (* list in reverse order so that dependencies get unfolded *)
@@ -18,3 +18,10 @@ Ltac serialize_deserialize_id_crush :=
   intros; deserializer_unfold;
   repeat rewrite ?app_assoc_reverse, ?serialize_deserialize_id;
   auto.
+
+(* Like Candy Crush if the candy was triangular. *)
+Ltac triangle_crush :=
+intros;
+deserializer_unfold;
+repeat rewrite ?app_assoc_reverse, ?serialize_deserialize_id, ?triangle;
+auto.
